\section{Матрицы — Матричные уравнения}

\begin{sagesilent}
    A = matrix(QQ, [[-2, 4, -6], [-1, 0, 2], [4, 4, 2]])
    B = matrix(QQ, [[2, 8, -3], [-2, 2, 4], [1, 0, 2]])
\end{sagesilent}

Дано уравнение:

$1/2 * X * \sage{A}^{T} - 3*E = 1/4 * \sage{B}^{2}$
~\\

Решение уравнения сводится к двум вариантам умножения:
~\\

\begin{minipage}{0.4\textwidth}
	$A*X = B$
	
	$A^{-1}* A*X = A^{-1}*B$
	
	$X = A^{-1}*B$
\end{minipage}
\hfill
\begin{minipage}{0.4\textwidth}
	$X*A=B$
	
	$X*A*A^{-1} = B*A^{-1}$
	
	$X = B*A^{-1}$
	
\end{minipage}

\begin{sagesilent}
	A = matrix(QQ, [[-2, 4, -6], [-1, 0, 2], [4, 4, 2]])
	B = matrix(QQ, [[2, 8, -3], [-2, 2, 4], [1, 0, 2]])
	E = matrix(QQ, [[3, 0, 0], [0, 3, 0], [0, 0, 3]])
	A = A.transpose() / 2
	B = B**2 / 4 + E
	X = B * A.inverse()
\end{sagesilent}

~\\

$X * \sage{A} = \sage{B}$

~\\

$X = \sage{X}$
